Added test cases and cleaned up code

verification/stringLinearSearch.dfy
@@ -1,36 +1,42 @@
+predicate inList(a: seq<seq<char>>, key: seq<char>)
+{
+    exists j :: 0 <= j < |a| && |a[j]| == |key| && a[j] == key
+}
+
 method findWord(a: array<seq<char>>, key: seq<char>) returns (idx: int)
     requires a != null
     ensures idx == -1 || 0 <= idx < a.Length
-    ensures idx == -1 <==> !(exists j::0<=j<a.Length && |a[j][..]| == |key| && a[j][..] == key)
-    ensures (0 <= idx < a.Length) <==> (exists j::0<=j<a.Length && |a[j][..]| == |key| && a[j][..] == key && j == idx)
+    ensures idx == -1 <==> !inList(a[..], key);
+    ensures (0 <= idx < a.Length) <==> (inList(a[..], key) && a[idx] == key)
 {
     idx := 0;
     while idx < a.Length && !(|a[idx][..]| == |key| && a[idx][..] == key)
     invariant 0 <= idx <= a.Length
     invariant forall i :: 0 <= i < idx ==> !(|a[i][..]| == |key| && a[i][..] == key)
-    {
+    {  
         idx := idx + 1;
     }
     if idx == a.Length { idx := -1; }
 }
 
-method Main() {
-    var list: array<seq<char>> := new seq<char>[3];
+method Test() {
+    var s1: seq<char> := ['a', 'b', 'c'];
+    var s2: seq<char> := ['d', 'e', 'f'];
+    var s3: seq<char> := ['g', 'h', 'i'];
 
-    var s1: seq<char> := ['x', 'y', 'z'];
-    var s2: seq<char> := ['a', 'b', 'c'];
-    var s3: seq<char> := ['d', 'e', 'f'];
+    var a: array<seq<char>> := new seq<char>[3];
+    a[0], a[1], a[2] := s1, s2, s3;
+
+    assert a[0] == s1;
+    assert a[1] == s2;
+    assert a[2] == s3;
 
     var key: seq<char> := ['a', 'b', 'c'];
+    var idx := findWord(a, key);
+    assert 0 <= idx < a.Length && a[idx] == key;
 
-    list[0], list[1], list[2] := s1, s2, s3;
-
-    assert list[0][..] == s1;
-    assert list[1][..] == s2;
-    assert list[2][..] == s3;
-    assert key == s2;
-    assert list[1][..] == key;
-
-    var idx := findWord(list, key);
-    assert 0 <= idx < list.Length ==> list[idx][..] == list[1][..];
+    key := ['x', 'y', 'z'];
+    idx := findWord(a, key);
+    assert key[0] == 'x' && key[1] == 'y' && key[2] == 'z';
+    assert idx == -1;
 }
